additions to stateful bigints

examples/stateful_bignum/neg_st.fst
@@ -5,17 +5,70 @@ open ST
 open IntLib
 open Bigint
 
-assume val neg:
-    b:bigint -> 
-    ST bigint
-      (requires (fun h -> 
-	(inHeap h b)
-       ))
-      (ensures (fun h0 c h1 ->
-	(inHeap h0 b)
-	/\ (inHeap h1 c)
-	/\ (getLength h1 c = getLength h0 b)
-	/\ (forall (i:nat). i < getLength h1 c
-	    ==> (getSize h0 b i = getSize h1 c i
-		/\ getValue h0 b i = getValue h1 c i))
-       ))
+val neg_aux :
+  b:bigint -> ghost_b:Seq.seq (tint ocaml63) -> ctr:nat ->
+  ST unit
+    (requires (fun h -> 
+      (inHeap h b)
+      /\ (ctr <= getLength h b)
+      /\ (Seq.length ghost_b = getLength h b)
+      /\ (forall (i:nat). i < ctr 
+	  ==> (getSize h b i = dfst (Seq.index ghost_b i)
+	      /\ getValue h b i = - (dsnd (Seq.index ghost_b i))))
+      /\ (forall (i:nat). (i >= ctr /\ i < getLength h b)
+	  ==> (getSize h b i = dfst (Seq.index ghost_b i)
+	      /\ getValue h b i = dsnd (Seq.index ghost_b i)))
+     ))
+    (ensures (fun h0 u h1 ->
+      (inHeap h1 b)
+      /\ (inHeap h0 b)
+      /\ (modifies !{Bigint63.data b} h0 h1)
+      /\ (Seq.length ghost_b = getLength h0 b)
+      /\ (ctr <= getLength h0 b)
+      /\ (getLength h0 b = getLength h1 b)
+      /\ (forall (i:nat). i < getLength h1 b
+	  ==> (getSize h1 b i = dfst (Seq.index ghost_b i)
+	      /\ getValue h1 b i = - (dsnd (Seq.index ghost_b i) )))
+     ))
+let rec neg_aux b ghost_b ctr =
+  match get_length b - ctr with
+  | 0 -> ()
+  | _ -> 
+     let bi = - (get b ctr) in
+     let h0 = erase (ST.get()) in
+     let size_bi = 
+       erase (getSize h0 b ctr) in
+     let bi = mk_tint b size_bi bi in
+     Bigint.updateBigint b ctr bi;
+     neg_aux b ghost_b (ctr+1)	    
+	   
+
+val neg:
+  b:bigint -> 
+  ST bigint
+    (requires (fun h -> 
+      (inHeap h b)
+      /\ (getLength h b > 0)
+     ))
+    (ensures (fun h0 c h1 ->
+      (inHeap h0 b)
+      /\ (getLength h0 b > 0)
+      /\ (inHeap h1 c)
+      /\ (modifies !{} h0 h1)
+      /\ (getLength h1 c = getLength h0 b)
+      /\ (forall (i:nat). i < getLength h1 c
+	  ==> (getSize h0 b i = getSize h1 c i
+	      /\ getValue h0 b i = - (getValue h1 c i)))
+     ))
+let neg b =
+  let h0 = erase (ST.get()) in
+  let c = Bigint.copy b in
+  let h0' = erase (ST.get()) in
+  //cut (modifies !{} h0 h0');
+  neg_aux c (Array.to_seq (Bigint63.data c)) 0;
+  let h1 = erase (ST.get()) in
+  cut (True /\ inHeap h1 c);
+  //cut (True /\ getLength h0 b = getLength h1 c);
+  //cut (modifies !{Bigint63.data c} h0' h1);
+  //cut (modifies!{} h0 h1);
+  c
